Refine_Imperative_HOL/Lib/Sepref_Misc.thy
@@ -1,12 +1,12 @@
 theory Sepref_Misc
 imports 
-  Refine_Monadic.Refine_Monadic
+  Refine_Monadic.Refine_Misc
   PO_Normalizer
   "List-Index.List_Index"
-  Separation_Logic_Imperative_HOL.Sep_Main
+(*  Separation_Logic_Imperative_HOL.Sep_Main *)
   Named_Theorems_Rev
   "HOL-Eisbach.Eisbach"
-  Separation_Logic_Imperative_HOL.Array_Blit
+(*  Separation_Logic_Imperative_HOL.Array_Blit *)
 begin
 
   hide_const (open) CONSTRAINT
